

Updates: Dependent Combinator Calculus

Alexandra Aiello

February 11, 2026

Current Iteration

```
abbrev Level := ℕ
```

```
inductive Expr where
```

```

| app  : Expr → Expr → Expr
| ty   : Level → Expr
| judge : Level → Expr
  -- ( $\alpha : \text{Type } m$ )  $\rightarrow \alpha \rightarrow \text{Prop}$ 
| Pi   : Expr
  -- ( $\text{Prop} \rightarrow \text{Prop}$ )  $\rightarrow (\text{Prop} \rightarrow \text{Prop} \rightarrow \text{Prop}) \rightarrow (\text{Type } 0)$ 
| vdash : Expr -- combine judgements into a judgment of an app
| prop  : Expr -- only inhabited by  $\vdash$  and :
-- fst, snd, comp - traversal combinators for Prop
| fst   : Expr
| snd   : Expr
| comp  : Expr
/-
  SK + I + C combinator from BCKW
-/
| const' : Level → Level → Expr
| const  : Level → Level → Expr
| flip   : Level → Level → Level → Expr
| both   : Level → Level → Level → Expr
| id     : Level → Expr
```

Step Relation

```
inductive IsStep : Expr → Expr → Prop
| id      : IsStep ((Expr.id m) _α x) x
| both    : IsStep ((both m n o) _α _β _γ x y z) ((x z) (y z))
| flip    : IsStep ((Expr.flip m n o) _α _β _γ x y z) (x z y)
| const'  : IsStep ((const' m n) _α _β x y) x
| comp    : IsStep ((f ∘ g) x) (f (g x))
| fst     : IsStep (fst (⊢ t_app judge_f judge_x)) judge_f
| snd     : IsStep (snd (⊢ t_app judge_f judge_x)) judge_x
| left    : IsStep f f'
| → IsStep (f x) (f' x)
| right   : IsStep x x'
| → IsStep (f x) (f x')
```

Inference Rules

```
inductive ValidJudgment : Expr → Prop
| app : ValidJudgment ((: 1) (Pi t_in t_out) f)
  → ValidJudgment ((: n) t_x x)
  → DefEq (t_in ((: 1) (Pi t_in t_out) f)) ((: n.succ) (Ty n) t_x)
  -- t_out decides what to do with the context and make a new judgment
  → ValidJudgment (t_out
    ((: 1) (Pi t_in t_out) f)
    ((: n) t_x x))

| parapp : ValidJudgment (⊢ ((: 1) (Ty 0) (Pi t_in t_out)) judge_inner_f judge_inner_x)
  → ValidJudgment ((: n) t_x x)
  → DefEq (t_in (⊢ ((: 1) (Ty 0) (Pi t_in t_out)) judge_inner_f judge_inner_x)) ((: n.succ) (Ty n) t_x)
  → ValidJudgment (t_out
    (⊢ ((: 1) (Ty 0) (Pi t_in t_out)) judge_inner_f judge_inner_x)
    ((: n) t_x x))
-- ... on next slide
```

Inference Rules (cont...)

```
-- ... ValidJudgment
/-
  Unclear how suspicious this is. See DefEq on the next slide.
  This could be easily refactored by matching the (: T e) e
  and only defeq-ing the type.
-/-
| defeq    : ValidJudgment j₁
  → DefEq j₁ j₂
  → ValidJudgment j₂
-/-
  Base combinator types. All point-free. Too many to fit on one slide.
-/-
| const : ValidJudgment ((: 1) (const.type m n) (const m n))
| both  : ValidJudgment ((: 1) (both.type m n o) (both m n o))
... -- more base combinator types
```

```
inductive DefEq : Expr → Expr → Prop
| refl      : DefEq a a
| step      : IsStep e e' → DefEq e e'
| trans     : DefEq e1 e2 → DefEq e2 e3 → DefEq e1 e3
| left      : DefEq f f' → DefEq (f x) (f' x)
| right     : DefEq x x' → DefEq (f x) (f x')
| vdash     : DefEq judge_app ((: m.succ) (Ty m) t_fx)
  → DefEq judge_f ((: n) t_f f)
  → DefEq judge_x ((: o) t_x x)
  → DefEq (⊢ judge_app judge_f judge_x) ((: m) t_fx (f x))
```

Combinator Types: Dependent K

```
def const.type (m n : Level) : Expr :=
  let  $\alpha$  := mk_assert_in (Ty m) m.succ
  -- takes  $\alpha$ , makes a new ( $\alpha \rightarrow$  Type  $n$ )
  let  $\beta$ . $\alpha$  := Expr.snd
  let  $\beta$ .const := ((const' 0 0) Prp Prp)  $\circ$  Expr.snd
  let  $\beta$ .const_out := (mk_assert_out (Ty n) n.succ)
  let  $\beta$  := (( $\lambda$  2) (Ty 1))  $\circ$  ((flip_pi  $\beta$ .const_out)  $\circ$   $\beta$ .const))

let  $\beta$ x := ((both 0 0 0)
  Prp
  ((const' 0 1) (Ty 0) Prp Prp)
  ((const' 0 1) (mk_arrow Prp Prp 0 0) Prp ((const' 0 1) (Ty 0) Prp))
  (( $\lambda$  ( $\lambda$  n.succ.succ) (Ty n.succ) (Ty n)))  $\circ$  (snd  $\circ$  fst))
  snd)

-- Inserts our type in ( $\lambda$  T (const  $\alpha$   $\beta$  x y)) this position.
let cpy := ((both 0 0 0)
  Prp
  ((const' 1 0) (Ty 0) Prp Prp)
  ((const' 1 0) (mk_arrow Prp (Ty 0) 0 1) Prp
    ((const' 1 0) (Ty 0) Prp
      (mk_arrow Prp (mk_arrow Prp Prp 0 0) 0 1))))
let out := (cpy ( $\lambda$   $\circ$  (snd  $\circ$  fst  $\circ$  fst)) ((id 0) Prp))

( $\Pi$  ((const' 0 0) Prp Prp (( $\lambda$  m.succ.succ) (Ty m.succ) (Ty m)))
  ( $\lambda$  ( $\lambda$  1) (Ty 0)
    ( $\Pi$   $\beta$ 
      ( $\lambda$  ( $\lambda$  1) (Ty 0) ( $\Pi$  (Expr.snd  $\circ$  Expr.fst) ( $\lambda$  ( $\lambda$  1) (Ty 0) ( $\Pi$   $\beta$ x out))))))
```


The Proof

```
theorem const_well_typed : ValidJudgment ((: m.succ) (Ty m)  $\alpha$ )  
  → ValidJudgment ((: 1) (mk_arrow  $\alpha$  (Ty n) m n.succ)  $\beta$ )  
  → ValidJudgment ((: m)  $\alpha$  x)  
  → ValidJudgment ((: n) ( $\beta$  x) y)  
  → ValidJudgment ((: m)  $\alpha$  ((const m n)  $\alpha$   $\beta$  x y)) := by  
  intro h_t_ $\alpha$  h_t_ $\beta$  h_t_x h_t_y  
  judge defeq, parapp, defeq, parapp, defeq, parapp, defeq, app, const  
  exact m  
  exact n  
  exact h_t_ $\alpha$   
  defeq step  
  step const'  
  defeq refl  
  exact h_t_ $\beta$   
  unfold mk_arrow  
  simp  
  defeq trans, step  
  step comp  
  defeq trans, right, step  
  step comp  
  defeq right, trans, step  
  ... -- too many steps to list on screen
```

The S Type

```
def both.type (m n o : Level) : Expr :=
  /-
    Same as in const.  $\alpha : \text{Type}$ ,  $\beta : \alpha \rightarrow \text{Type}$ 
  -/
  let  $\alpha := \text{mk\_assert\_in } (\text{Ty } m) \text{ m.succ}$ 

  -- takes  $\alpha$ , makes a new  $(\alpha \rightarrow \text{Type } n)$ 
  let  $\beta.\alpha := \text{Expr.snd}$ 
  let  $\beta.\text{const} := ((\text{const' } 0 \ 0) \text{ Prp Prp}) \circ \beta.\alpha$ 
  let  $\beta.\text{const\_out} := (\text{mk\_assert\_out } (\text{Ty } n) \text{ n.succ})$ 
  let  $\beta := ((\text{(: } 2) \text{ (Ty } 1)}) \circ ((\text{flip\_pi } \beta.\text{const\_out}) \circ \beta.\text{const}))$ 

  let  $y := ((\text{both\_nondep Prp (mk\_arrow Prp Prp } 0 \ 0) \text{ (Ty } 0) \ 0 \ 1 \ 1)$ 
    ( $\text{Pi } \circ (\text{snd } \circ \text{fst})$ )
    ( $((\text{!- } ((\text{(: } 1) \text{ (Ty } 0)))) \circ$ 
      ( $\text{flip\_pi}$ 
        ( $\text{mk\_assert\_out } (\text{Ty } o) \text{ o.succ}$ )
        ( $((\text{flip\_comp snd}) \circ ((\text{!- } ((\text{(: } n.\text{succ.succ}) \text{ (Ty } n.\text{succ}) \text{ (Ty } n)))) \circ \text{Expr.snd}))))))$ 
    )
  let  $x.\text{mk\_y\_xy} := (((\text{comp !- } ((\text{(: } o.\text{succ.succ}) \text{ (Ty } o.\text{succ}) \text{ (Ty } o)))) \circ$ 
    ( $((\text{flip\_comp snd}) \circ !- ((\text{(: } o.\text{succ.succ}) \text{ (Ty } o.\text{succ}) \text{ (Ty } o)))) \circ \text{Expr.snd}$ )
  let  $x := ((\text{both\_nondep Prp (mk\_arrow Prp Prp } 0 \ 0) \text{ (Ty } 0) \ 0 \ 1 \ 1)$ 
    ( $\text{Pi } \circ (\text{snd } \circ \text{fst } \circ \text{fst})$ )
    ( $((\text{!- } ((\text{(: } 1) \text{ (Ty } 0)))) \circ$ 
      ( $((\text{both\_nondep Prp (mk\_arrow Prp Prp } 0 \ 0) \text{ (Ty } 0) \ 0 \ 1 \ 1)$ 
        ( $((\text{flip\_comp snd}) \circ ((\text{!- } ((\text{(: } n.\text{succ.succ}) \text{ (Ty } n.\text{succ}) \text{ (Ty } n)))) \circ (\text{Expr.snd } \circ \text{fst}))))$ 
         $x.\text{mk\_y\_xy}))$ 
    )
  let  $y := ((\text{both\_nondep Prp (mk\_arrow Prp Prp } 0 \ 0) \text{ (Ty } 0) \ 0 \ 1 \ 1)$ 
    ( $\text{Pi } \circ (\text{snd } \circ \text{fst } \circ \text{fst } \circ \text{fst})$ ) -- ( $x : \alpha$ )
    ( $((\text{!- } ((\text{(: } n.\text{succ.succ}) \text{ (Ty } n.\text{succ}) \text{ (Ty } n)))) \circ (\text{Expr.snd } \circ \text{fst } \circ \text{fst}))))$ 
  ( $\text{Pi } \alpha \text{ (ret\_pi}$ 
    ( $\text{Pi } \beta \text{ (ret\_pi}$ 
      ( $\text{Pi } \gamma \text{ (ret\_pi}$ 
```


Summary of Past Iterations

Distinct Iterations of the Calculus

| Name | Main Feature | Meta Combinators?* | Uncurried Types? | Types are Well-Typed? |
|----------------------|--------------------------------|--------------------|-------------------|--|
| <i>SKM</i> | Reflection | Yes | No | No |
| <i>SKII</i> | II Combinator | Yes | No | No |
| <i>SKI</i> | (Γ, Δ) registers | No | Yes | Barely. Couldn't handle random edge cases. |
| List Calculus | Extremely minimal kernel | No | Barely well-typed | Barely well-typed |
| Sigma interpretation | Sigma type is data encoding II | No | No | Probably |

Figure: *Meta combinators result in a huge tree. Each meta combinator has a type.

The Ideal Dependent Combinator Calculus

- Use (Γ, Δ) registers.
- Condense π , next , read into one rule (equivalence proven ):
 - Very small kernel
- Pair interpretation: $\Gamma[n]$ is a nested pair. Same eval rules as in (Γ, Δ) , but a new well-typed meaning.
- nil combinator: downgrades a term to a type.
 - Useful for arguments like $\alpha : \text{Type } n$
- Core calculus is the typical SK combinators

Central Thesis: The Sigma-Curry Correspondence

- Combinator types are much easier to form with all arguments in scope (“uncurried”)
- I demonstrate [▶ here](#) that `Sigma.snd` projection is equivalent to function application
- Treating the future application as *data* makes forming types much simpler
- We can capture projection of `fst`, `snd`, application, and many more with a single reduction rule

Research Questions: Sigma-Curry Correspondence

Hypotheses: Sigma-Curry Correspondence

- Should we internalize π projection in $::[a, b]$, or should we have $::[fst, snd]$ combinators? **Yes, internalize projection!**
 - Can we derive fst ? **Yes!**
 - Can we derive snd ? **Yes!**
 - Can we fully emulate the old π combinator with a projector argument? **Yes!**
- Can we derive application from π projection? **Yes!**
- Can we derive S from both $+ \pi(id)$? **Yes!**
- Choose between $fst + snd$ or π list projection combinator. **Answered above.**
 - Intuition says fst and snd , since they would have simpler types. **Can derive snd and fst .**
- Can we derive nil from $::[x, xs] f$?

Research Questions AST

```
inductive Expr where
| app : Expr → Expr → Expr
| cons : Expr → Expr → Expr
| π : Expr
| fst : Expr | snd : Expr
| both : Expr
| const : Expr | const' : Expr
| id : Expr | nil : Expr | ty : Expr

inductive IsStepStar { rel : Expr → Expr → Prop } : Expr → Expr → Prop
| refl : IsStepStar e e
| trans : rel e1 e2
  → IsStepStar e2 e3
  → IsStepStar e1 e3
```

Figure: I have omitted universe levels for our research question proofs.

Research Questions: Sigma-Curry Correspondence
fst and snd can be condensed into one rule

Single-Step Reduction for Projection Derivations

inductive IsStep : Expr → Expr → Prop

```
| sapp : IsStep (.app :: [x, f], fn) (.app (.app fn f) x)
| fst  : IsStep (\$ fst, _α, _β, fn, :: [x, f]) (\$ fn, x)
| snd  : IsStep (\$ snd, _α, _β, fn, :: [x, f]) (\$ fn, f, x)
| nil  : IsStep (\$ nil, α, x) α
| id   : IsStep (\$ Expr.id, _α, x) x
| const' : IsStep (\$ const', _α, _β, x, y) x
| left  : IsStep f f'
→ IsStep (\$ f, x) (\$ f', x)
| right : IsStep x x'
→ IsStep (\$ f, x) (\$ f, x')
```

Deriving the Explicit fst Combinator

```
/-
  fst  $\alpha$   $\beta$  fn ::[head, tail] = fn head =
    ::[head, tail] fn =* fn head
-/
theorem fst_der (head tail fn : Expr) : IsStep
  (\$ fst, _ $\alpha$ , _ $\beta$ , fn, ::[head, tail]) (\$ fn, head)  $\leftrightarrow$ 
  (@IsStepStar IsStep) (\$ ::[head, tail],
    (\$ const', ::[ $\beta$ , (\$ nil,  $\beta$ )],  $\alpha$ , fn)) (\$ fn, head) := by
  constructor
  intro h_step; cases h_step
  apply IsStepStar.trans; apply IsStep.sapp
  apply IsStepStar.trans; apply IsStep.left
  apply IsStep.const'; apply IsStepStar.refl
  intro h_step; cases h_step
  case mpr.trans e2 h_step h_trans  $\Rightarrow$ 
    cases h_trans; apply IsStep.fst
    apply IsStep.fst
```

Deriving the Explicit snd Combinator

```
/-  
  snd  $\alpha$   $\beta$  fn ::[head, tail] = ::[head, tail] fn  
  = fn tail head  
-/
```

theorem snd_der (head tail fn : Expr) : IsStep
 (\\$ snd, _ α , _ β , fn, ::[head, tail]) (\\$ fn, tail, head) \leftrightarrow
 (@IsStepStar IsStep) (\\$::[head, tail], fn) (\\$ fn, tail, head) := by
 constructor
 intro h_step; cases h_step
 apply IsStepStar.trans; apply IsStep.sapp
 apply IsStepStar.refl
 case mp.right a \Rightarrow
 cases a
 intro h_step
 cases h_step
 apply IsStep.snd

Research Questions: Sigma-Curry Correspondence
Sigma projection is equivalent to application

Single-Step Reduction for Sigma Equivalence Proofs

```
inductive IsStep : Expr → Expr → Prop
| sapp  : IsStep ($ :: [x, f], fn) ($ fn, f, x)
| nil   : IsStep ($ nil, α, x) α
| id    : IsStep ($ Expr.id, _α, x) x
| const' : IsStep ($ const', _α, _β, x, y) x
| const  : IsStep ($ const, _α, _β, x, y) x
/- f and g order is flipped here compared to S.
   both f g x = ::[(f x), (g x)]
   both f g x id = id (g x) (f x) -/
| both  : IsStep ($ both, _α, _β, _γ, f, g, x)
  :: [($f, x), ($g, x)]
| left  : IsStep f f'
  → IsStep ($ f, x) ($ f', x)
| right : IsStep x x'
  → IsStep ($ f, x) ($ f, x')
```

All Function Applications have corresponding Sigma Projections

```
/-  
(f x) = e' implies (::[x, f] (id t_f)) = e'  
-/  
theorem app_imp_proj (t_f f x : Expr) : (@IsStepStar IsStep)  
  (\$ f, x) e' → (@IsStepStar IsStep)  
  (\$ ::[x, f], (\$ id, t_f)) e' := by  
  intro h_step  
  cases h_step  
  apply IsStepStar.trans; apply IsStep.sapp  
  apply IsStepStar.trans; apply IsStep.left  
  apply IsStep.id; apply IsStepStar.refl  
  apply IsStepStar.trans; apply IsStep.sapp  
  apply IsStepStar.trans; apply IsStep.left  
  apply IsStep.id; apply IsStepStar.trans  
  repeat assumption
```


All Function Applications are $=_\beta$ Sigma Projection

```
/-  
(f x)  $\beta$ = (::[x, f] (id t_f))  
-/  
theorem apps_are_proj (t_f f x : Expr) : (@IsBetaEq IsStep)  
  (\$ f, x) (\$ ::[x, f], (\$ id, t_f)) := by  
  apply IsBetaEq.symm; apply IsBetaEq.trans  
  apply IsBetaEq.rel; apply IsStep.sapp  
  apply IsBetaEq.trans; apply IsBetaEq.rel  
  apply IsStep.left; apply IsStep.id  
  apply IsBetaEq.refl
```

Research Questions: Sigma-Curry Correspondence
Deriving the S combinator from both $+$ and projection

S combinator = $id \circ both$

```
theorem s_both_app_beq ( $\alpha \beta \gamma f g x : Expr'$ ) : (@IsBetaEq IsStep)
  ( $\$' s, \alpha, \beta, \gamma, f, g, x$ )
  ( $\$' (\$' both, \alpha, \beta, \gamma, g, f, x), (\$' id, (\$' \beta, z))) := by
  apply IsBetaEq.trans; apply IsBetaEq.rel
  apply IsStep.s; apply IsBetaEq.symm
  apply IsBetaEq.trans; apply IsBetaEq.rel
  apply IsStep.left; apply IsStep.both
  apply IsBetaEq.trans; apply IsBetaEq.rel
  apply IsStep.sapp; apply IsBetaEq.trans
  apply IsBetaEq.rel; apply IsStep.left
  apply IsStep.id; apply IsBetaEq.refl$ 
```

Figure: This proof uses an extended AST with the S combinator for the purposes of this equivalence. Note that the order of f and g are flipped between S and $both$, since $both$ is sigma-native.

Research Questions: (Γ, Δ) Contexts

Very Dependent Types

- $:: [x, xs]$ represents a term. It is computationally relevant. What is the equivalent for types?
- $x : F\ x$: very dependent types, such as this one featured in Altenkirch et al. [Alt+23] might be useful. Not helpful—use Π with clever inference and reduction rules.
- Since our sigma terms encode application as data, we can easily traverse the “context”. List context is also unnecessary, seemingly. See [here](#).
- $\Sigma\ t_in\ t_out : \text{Type}$
- To infer domain / codomain:
 $((f : \Sigma\ T\ \alpha\ T\beta) (x : \alpha)) : ((T :: [x, f])\ \pi))$
 - Problem: to project either component, we must know α and β .
- Can we do better with
 $((f : \Sigma\ T) (x : \alpha)) : ((T :: [x, \Sigma\ T])\ \text{snd}))?$
- Since $\Sigma\ T$ is a **Type**, the user cannot force evaluation. Only the kernel can.

```

inductive Expr where
| app      : Expr → Expr → Expr
/- List-like objects
   They come with built-in projection.
   They are the mirror image of application "as data". -/
| cons     : Expr → Expr → Expr
/-
   ::[x, xs] lists are a special case. They are the mirror
   image of application as data. They internalize a projector
   argument  $\pi$ .
-/
| Prod     : Expr → Expr → Expr
/-
   Our representation of curried function types.
    $\Pi t_{in} t_{out}$ 
-/
| Pi       : Expr → Expr → Expr
| both     : Expr
| const    : Expr
| const'   : Expr
| id       : Expr
-- downgrades a term to a type
| nil      : Expr
| ty       : Expr

```